Major Improvements
- The semantics was updated to be compliant with a more recent version of Solidity (v0.8.25).
- In addition to external functions it now also supports internal functions.
- In addition to the verification of invariants, it now also supports the verification of (multiple) pre/post-conditions for functions.
- Type consistency is added as pre-condition for functions.

Solidity.thy
@@ -1,22 +1,27 @@
 theory Solidity
-imports State_Monad State
+imports State_Monad State "Finite-Map-Extras.Finite_Map_Extras"
 begin
 
-datatype ('a::address) rvalue =
-  Storage id "('a::address) valtype list" |
-  Memory location |
-  Calldata id "('a::address) valtype list" |
-  Value (vt: "('a::address) valtype") |
+section \<open>Value types\<close>
+
+datatype ('a) rvalue =
+  Storage "'a valtype pointer option" |
+  Memory (memloc: location) |
+  Calldata "'a valtype pointer option" |
+  Value (vt: "'a valtype") |
   Empty
 
 definition kdbool where
   "kdbool = Value \<circ> Bool"
 
 definition kdSint where
-  "kdSint \<equiv> Value \<circ> Sint"
+  "kdSint \<equiv> Value \<circ> Uint"
 
 definition kdAddress where
   "kdAddress = Value \<circ> Address"
+
+definition kdBytes where
+  "kdBytes \<equiv> Value \<circ> Bytes"
 
 fun lift_value_unary::"(('a::address) valtype \<Rightarrow> ('a::address) valtype option) \<Rightarrow> ('a::address) rvalue \<Rightarrow> ('a::address) rvalue option" where
   "lift_value_unary op (rvalue.Value v) = op v \<bind> Some \<circ> rvalue.Value"
@@ -56,8 +61,29 @@ definition kdminus_safe where
 definition kdmult where
   "kdmult = lift_value_binary vtmult"
 
+definition kdmult_safe where
+  "kdmult_safe = lift_value_binary vtmult_safe"
+
 definition kdmod where
   "kdmod = lift_value_binary vtmod"
+
+definition kdbytes_index where
+  "kdbytes_index = lift_value_binary vtbytes_index"
+
+definition kdbytes_and where
+  "kdbytes_and = lift_value_binary vtbytes_and"
+
+definition kdbytes_or where
+  "kdbytes_or = lift_value_binary vtbytes_or"
+
+definition kdbytes_xor where
+  "kdbytes_xor = lift_value_binary vtbytes_xor"
+
+definition kdbytes_not where
+  "kdbytes_not = lift_value_unary vtbytes_not"
+
+definition kdbytes_cast where
+  "kdbytes_cast m = lift_value_unary (vtbytes_cast m)"
 
 type_synonym 'a expression_monad = "('a rvalue, ex, 'a state) state_monad"
 
@@ -85,63 +111,84 @@ primrec lfold :: "('a::address) expression_monad list \<Rightarrow> (('a::addres
         return (l' # ls)
       }"
 
-locale Keccak256 =
-  fixes keccak256::"('a::address) rvalue \<Rightarrow> ('a::address) rvalue"
-  assumes "\<And>x y. keccak256 x = keccak256 y \<Longrightarrow> x = y"
+section \<open>Constants\<close>
+
+definition bool_monad where
+  "bool_monad = return \<circ> kdbool"
+
+definition true_monad::"('a::address) expression_monad" ("\<langle>T\<rangle>")  where
+  "true_monad = bool_monad True"
+
+definition false_monad::"('a::address) expression_monad"("\<langle>F\<rangle>")  where
+  "false_monad = bool_monad False"
+
+definition sint_monad ("(\<langle>sint\<rangle> _)" [70] 69) where
+  "sint_monad = return \<circ> kdSint"
+
+definition bytes_monad where
+  "bytes_monad n xs  = (if n \<notin> {1..<33} \<or> n \<noteq> length xs then throw Err else return (kdBytes xs))"
+
+definition address_monad where
+  "address_monad = return \<circ> kdAddress"
+
+definition bytes_monad2 where
+  "bytes_monad2 = return \<circ> kdBytes"
+
+locale Contract =
+  fixes this :: "'a::address" (*address of executing contract*)
 begin
 
-definition keccak256_monad::"('a::address) expression_monad \<Rightarrow> ('a::address) expression_monad" where
+definition this_monad where
+  "this_monad = address_monad this"
+
+end
+
+locale Method =
+  fixes msg_sender :: "'a::address" (*address of calling contract*)
+    and msg_value :: "256 word" (*money send*)
+    and timestamp :: "256 word" (*time stamp of a block*)
+  assumes sender_neq_null: "msg_sender \<noteq> null"
+  assumes less_bound: "unat timestamp < 2^256"
+begin
+
+definition sender_monad  ("\<langle>sender\<rangle>") where
+  "sender_monad = address_monad msg_sender"
+
+definition value_monad ("\<langle>value\<rangle>") where
+  "value_monad = sint_monad msg_value"
+
+definition block_timestamp_monad ("\<langle>stamp\<rangle>") where
+  "block_timestamp_monad = sint_monad timestamp"
+
+definition null_monad  ("\<langle>nul\<rangle>") where
+  "null_monad = address_monad null"
+
+end
+
+locale Keccak256 =
+  fixes keccak256::"('a::address) rvalue \<Rightarrow> ('a::address) rvalue"
+  and encodeABI::"('a::address) rvalue list \<Rightarrow> ('a::address) rvalue"
+  assumes "\<And>x y. keccak256 x = keccak256 y \<Longrightarrow> x = y"
+(*      and "\<And>xs ys. encodeABI xs = encodeABI ys \<Longrightarrow> xs = ys"*)
+begin
+
+definition keccak256_monad::"('a::address) expression_monad \<Rightarrow> ('a::address) expression_monad" ("\<langle>keccak256\<rangle>") where
   "keccak256_monad m = 
     do {
       v \<leftarrow> m;
       return (keccak256 v)
     }"
 
-end
-
-locale Contract =
-  fixes this :: "'a::address" (*address of executing contract*)
-
-begin
-
-definition storage_update:: "id \<Rightarrow> ('a::address) sdata \<Rightarrow> ('a::address) state \<Rightarrow> ('a::address) state" where
-  "storage_update i d s = s\<lparr>Storage := (state.Storage s) (this := (state.Storage s this) (i := d))\<rparr>"
-
-abbreviation balance_update:: "nat \<Rightarrow> ('a::address) state \<Rightarrow> ('a::address) state" where
-  "balance_update \<equiv> balances_update this"
-
-definition inv:: "'a rvalue \<times> ('a::address) state + ex \<times> ('a::address) state \<Rightarrow> (('a::address) state \<Rightarrow> bool) \<Rightarrow> (('a::address) state \<Rightarrow> bool) \<Rightarrow> bool" where
-  "inv r P Q \<equiv> (case r of Inl a \<Rightarrow> P (snd a)
-                        | Inr a \<Rightarrow> Q (snd a))"
-
-definition inv_state:: "((id \<Rightarrow> ('a::address) sdata) \<times> nat \<Rightarrow> bool) \<Rightarrow> ('a::address) state \<Rightarrow> bool"
-  where "inv_state i s = i (state.Storage s this, state.Balances s this)"
+definition encodeABI_monad::"('a::address) expression_monad list \<Rightarrow> ('a::address) expression_monad" ("\<langle>encodeABI\<rangle>") where
+  "encodeABI_monad ms =
+    do {
+      xs \<leftarrow> mfold ms;
+      return (encodeABI xs)
+    }"
 
 end
 
-section \<open>Expressions\<close>
-
-subsection \<open>Constants\<close>
-
-definition bool_monad where
-  "bool_monad = return \<circ> kdbool"
-
-definition true_monad::"('a::address) expression_monad" where
-  "true_monad = bool_monad True"
-
-definition false_monad::"('a::address) expression_monad" where
-  "false_monad = bool_monad False"
-
-definition sint_monad where
-  "sint_monad = return \<circ> kdSint"
-
-definition address_monad where
-  "address_monad = return \<circ> kdAddress"
-
-definition (in Contract) this_monad where
-  "this_monad = address_monad this"
-
-subsection \<open>Unary Operations\<close>
+section \<open>Unary Operations\<close>
 
 definition lift_unary_monad ::"(('a::address) rvalue \<Rightarrow> ('a::address) rvalue option) \<Rightarrow> ('a::address) expression_monad \<Rightarrow> ('a::address) expression_monad" where
   "lift_unary_monad op lm = 
@@ -151,10 +198,10 @@ definition lift_unary_monad ::"(('a::address) rvalue \<Rightarrow> ('a::address)
       return val
     }"
 
-definition not_monad::"('a::address) expression_monad \<Rightarrow> ('a::address) expression_monad" where
+definition not_monad::"('a::address) expression_monad \<Rightarrow> ('a::address) expression_monad" ("\<langle>\<not>\<rangle> _" 65) where
   "not_monad = lift_unary_monad kdnot"
 
-subsection \<open>Binary Operations\<close>
+section \<open>Binary Operations\<close>
 
 definition lift_op_monad::"(('a::address) rvalue \<Rightarrow> ('a::address) rvalue \<Rightarrow> ('a::address) rvalue option) \<Rightarrow> ('a::address) expression_monad \<Rightarrow> ('a::address) expression_monad \<Rightarrow> ('a::address) expression_monad" where
   "lift_op_monad op lm rm = 
@@ -193,7 +240,7 @@ lemma lift_op_monad_simp5:
     shows "execute (lift_op_monad op lm rm) s = execute (option Err (K (op lv rv))) s''"
   unfolding lift_op_monad_def by (simp add: execute_simps assms)
 
-definition equals_monad where
+definition equals_monad (infixl "\<langle>=\<rangle>" 65) where
   "equals_monad = lift_op_monad kdequals"
 
 lemma equals_monad_simp1[execute_simps]:
@@ -224,50 +271,68 @@ lemma equals_monad_simp5[execute_simps]:
     shows "execute (equals_monad lm rm) s = execute (option Err (K (kdequals lv rv))) s''"
   unfolding equals_monad_def by (rule lift_op_monad_simp5[OF assms])
 
-definition less_monad where
+definition less_monad (infixl "\<langle><\<rangle>" 65) where
   "less_monad = lift_op_monad kdless"
 
-definition and_monad where
+definition and_monad (infixl "\<langle>\<and>\<rangle>" 55) where
   "and_monad = lift_op_monad kdand"
 
-definition or_monad where
+definition or_monad (infixl "\<langle>\<or>\<rangle>" 54) where
   "or_monad = lift_op_monad kdor"
 
 definition plus_monad::"('a::address) expression_monad \<Rightarrow> ('a::address) expression_monad \<Rightarrow> ('a::address) expression_monad" where
   "plus_monad = lift_op_monad kdplus"
 
-definition plus_monad_safe::"('a::address) expression_monad \<Rightarrow> ('a::address) expression_monad \<Rightarrow> ('a::address) expression_monad" where
+definition plus_monad_safe::
+  "('a::address) expression_monad \<Rightarrow> ('a::address) expression_monad \<Rightarrow> ('a::address) expression_monad"
+  (infixl "\<langle>+\<rangle>" 65)
+where
   "plus_monad_safe = lift_op_monad kdplus_safe"
 
 definition minus_monad::"('a::address) expression_monad \<Rightarrow> ('a::address) expression_monad \<Rightarrow> ('a::address) expression_monad" where
   "minus_monad = lift_op_monad kdminus"
 
-definition minus_monad_safe::"('a::address) expression_monad \<Rightarrow> ('a::address) expression_monad \<Rightarrow> ('a::address) expression_monad" where
+definition minus_monad_safe::"('a::address) expression_monad \<Rightarrow> ('a::address) expression_monad \<Rightarrow> ('a::address) expression_monad" (infixl "\<langle>-\<rangle>" 65) where
   "minus_monad_safe = lift_op_monad kdminus_safe"
 
 definition mult_monad::"('a::address) expression_monad \<Rightarrow> ('a::address) expression_monad \<Rightarrow> ('a::address) expression_monad" where
   "mult_monad = lift_op_monad kdmult"
 
-definition mod_monad::"('a::address) expression_monad \<Rightarrow> ('a::address) expression_monad \<Rightarrow> ('a::address) expression_monad" where
+definition mult_monad_safe::"('a::address) expression_monad \<Rightarrow> ('a::address) expression_monad \<Rightarrow> ('a::address) expression_monad" (infixl "\<langle>*\<rangle>" 65) where
+  "mult_monad_safe = lift_op_monad kdmult_safe"
+
+definition mod_monad::"('a::address) expression_monad \<Rightarrow> ('a::address) expression_monad \<Rightarrow> ('a::address) expression_monad" (infixl "\<langle>%\<rangle>" 65) where
   "mod_monad = lift_op_monad kdmod"
 
-subsection \<open>Require\<close>
+definition bytes_index_monad where
+  "bytes_index_monad = lift_op_monad kdbytes_index"
 
-definition require_monad::"('a::address) expression_monad \<Rightarrow> ('a::address) expression_monad" where
-  "require_monad em = 
-    do {
-      e \<leftarrow> em;
-      if e = kdbool True then return Empty else throw Err
-    }"
+definition bytes_and_monad where
+  "bytes_and_monad = lift_op_monad kdbytes_and"
 
-subsection \<open>Store Lookups\<close>
+definition bytes_or_monad where
+  "bytes_or_monad = lift_op_monad kdbytes_or"
 
-definition (in Contract) storeLookup::"id \<Rightarrow> ('a::address) expression_monad list \<Rightarrow> ('a::address) expression_monad" where
+definition bytes_xor_monad where
+  "bytes_xor_monad = lift_op_monad kdbytes_xor"
+
+definition bytes_not_monad where
+  "bytes_not_monad = lift_unary_monad kdbytes_not"
+
+definition bytes_cast_monad where
+  "bytes_cast_monad m = lift_unary_monad (kdbytes_cast m)"
+
+section \<open>Store Lookups\<close>
+
+definition (in Contract) storeLookup::
+  "id \<Rightarrow> ('a::address) expression_monad list \<Rightarrow> ('a::address) expression_monad"
+  ("(_ ~\<^sub>s _)" [100, 100] 70) 
+where
   "storeLookup i es =
     do {
       is \<leftarrow> lfold es;
       sd \<leftarrow> option Err (\<lambda>s. slookup is (state.Storage s this i));
-      if sdata.is_Value sd then return (rvalue.Value (sdata.vt sd)) else return (rvalue.Storage i is)
+      if storage_data.is_Value sd then return (rvalue.Value (storage_data.vt sd)) else return (rvalue.Storage (Some \<lparr>Location=i, Offset= is\<rparr>))
     }"
 
 definition (in Contract) storeArrayLength::"id \<Rightarrow> ('a::address) expression_monad list \<Rightarrow> ('a::address) expression_monad" where
@@ -277,18 +342,104 @@ definition (in Contract) storeArrayLength::"id \<Rightarrow> ('a::address) expre
       sd \<leftarrow> option Err (\<lambda>s. slookup is (state.Storage s this i));
       storage_check sd
         (K (throw Err))
-        (\<lambda>sa. return (rvalue.Value (Sint (of_nat (length (sdata.ar sd))))))
+        (\<lambda>sa. return (rvalue.Value (Uint (of_nat (length (storage_data.ar sd))))))
         (K (throw Err))
     }"
 
-section \<open>Statements\<close>
+definition (in Contract) storeArrayLengthSafe::"id \<Rightarrow> ('a::address) expression_monad list \<Rightarrow> ('a::address) expression_monad" where
+  "storeArrayLengthSafe i es =
+    do {
+      is \<leftarrow> lfold es;
+      sd \<leftarrow> option Err (\<lambda>s. slookup is (state.Storage s this i));
+      storage_check sd
+        (K (throw Err))
+        (\<lambda>sa. (if length (storage_data.ar sd) < 2^256 then return (Value (Uint (word_of_nat (length (storage_data.ar sd))))) else throw Err))
+        (K (throw Err))
+    }"
 
-definition skip_monad:: "('a rvalue, ex, ('a::address) state) state_monad" where
+
+section \<open>Stack Lookups\<close>
+
+definition stack_check where
+  "stack_check i kf mf cf cp sf sp =
+    do {
+      k \<leftarrow> applyf Stack;
+      case k $$ i of
+        Some x \<Rightarrow>
+          (case x of
+            kdata.Value v \<Rightarrow> kf v
+          | kdata.Storage (Some p) \<Rightarrow> sf (Location p) (Offset p)
+          | kdata.Storage None \<Rightarrow> sp
+          | kdata.Memory l \<Rightarrow> mf l
+          | kdata.Calldata (Some p) \<Rightarrow> cf (Location p) (Offset p)
+          | kdata.Calldata None \<Rightarrow> cp)
+      | None \<Rightarrow> throw Err
+    }"
+
+definition(in Contract) stackLookup::
+  "id \<Rightarrow> ('a::address) expression_monad list \<Rightarrow> ('a::address) expression_monad"
+  ("(_ ~ _)" [1000, 0] 70)
+where
+  "stackLookup i es =
+    do {
+      is \<leftarrow> lfold es;
+      stack_check i
+        (\<lambda>k. return (Value k))
+        (\<lambda>l. do {
+          l' \<leftarrow> option Err (\<lambda>s. mlookup (state.Memory s) is l);
+          md  \<leftarrow> option Err (\<lambda>s. state.Memory s $ l');
+          if mdata.is_Value md then return (rvalue.Value (mdata.vt md)) else return (rvalue.Memory l')
+        })
+        (\<lambda>l xs. do {
+          sd \<leftarrow> option Err (\<lambda>s. state.Calldata s $$ l \<bind> clookup (xs@is));
+          if call_data.is_Value sd then return (rvalue.Value (call_data.vt sd)) else return (rvalue.Calldata (Some \<lparr>Location=l, Offset=xs@is\<rparr>))
+        })
+        (
+          return (rvalue.Calldata None)
+        )
+        (\<lambda>l xs. do {
+          sd \<leftarrow> option Err (\<lambda>s. slookup (xs@is) (state.Storage s this l));
+          if storage_data.is_Value sd then return (rvalue.Value (storage_data.vt sd)) else return (rvalue.Storage (Some \<lparr>Location=l, Offset=xs@is\<rparr>))
+        })
+        (
+          return (rvalue.Storage None)
+        )
+    }"
+
+definition(in Contract) arrayLength::"id \<Rightarrow> ('a::address) expression_monad list \<Rightarrow> ('a::address) expression_monad" where
+  "arrayLength i es =
+    do {
+      is \<leftarrow> lfold es;
+      stack_check i
+        (K (throw Err))
+        (\<lambda>l. do {
+          l' \<leftarrow> option Err (\<lambda>s. mlookup (state.Memory s) is l);
+          md  \<leftarrow> option Err (\<lambda>s. state.Memory s $ l');
+          if mdata.is_Array md then return (rvalue.Value (Uint (of_nat (length (mdata.ar md))))) else throw Err
+        })
+        (\<lambda>l xs. do {
+          sd \<leftarrow> option Err (\<lambda>s. state.Calldata s $$ l \<bind> clookup (xs@is));
+          if call_data.is_Array sd then return (rvalue.Value (Uint (of_nat (length (call_data.ar sd))))) else throw Err
+        })
+        (throw Err)
+        (\<lambda>l xs. do {
+          sd \<leftarrow> option Err (\<lambda>s. slookup (xs@is) (state.Storage s this l));
+          if storage_data.is_Array sd then return (rvalue.Value (Uint (of_nat (length (storage_data.ar sd))))) else throw Err
+        })
+        (throw Err)
+    }"
+
+section \<open>Skip\<close>
+
+definition skip_monad:: "('a rvalue, ex, ('a::address) state) state_monad" ("\<langle>skip\<rangle>") where
 "skip_monad = return Empty"
 
-subsection \<open>Conditionals\<close>
+section \<open>Conditionals\<close>
 
-definition cond_monad:: "('a::address) expression_monad \<Rightarrow> ('a::address) expression_monad \<Rightarrow> ('a::address) expression_monad \<Rightarrow> ('a::address) expression_monad" where
+definition cond_monad::
+  "('a::address) expression_monad \<Rightarrow> ('a::address) expression_monad \<Rightarrow> ('a::address) expression_monad \<Rightarrow> ('a::address) expression_monad"
+  ("(IF _/ THEN _/ ELSE _)"  [0, 0, 61] 61)
+where
 "cond_monad bm mt mf = 
   do {
     b \<leftarrow> equals_monad bm true_monad;
@@ -331,128 +482,100 @@ lemma execute_cond_monad_simp4[execute_simps]:
   shows "execute (cond_monad bm mt mf) s = NT"
   unfolding cond_monad_def by (simp add: execute_simps assms)
 
-subsection \<open>Assignments\<close>
+section \<open>Require/Assert\<close>
+
+definition require_monad::"('a::address) expression_monad \<Rightarrow> ('a::address) expression_monad" where
+  "require_monad em = 
+    do {
+      e \<leftarrow> em;
+      if e = kdbool True then return Empty else throw Err
+    }"
+
+definition assert_monad :: "('a::address) expression_monad \<Rightarrow> ('a::address) expression_monad" ("\<langle>assert\<rangle>") where
+ "assert_monad bm = 
+    cond_monad bm (return Empty) (throw Err)"
+
+section \<open>Stack Assign\<close>
 
 definition my_update_monad:: "(('a::address) state \<Rightarrow> 'b) \<Rightarrow> (('c \<Rightarrow> 'd) \<Rightarrow> ('a::address) state \<Rightarrow> ('a::address) state) \<Rightarrow> ('b \<Rightarrow> 'd option) \<Rightarrow> 'a expression_monad" where
   "my_update_monad s u f = option Err (\<lambda>s'. f (s s')) \<bind> modify \<circ> u \<circ> K \<bind> K (return Empty)"
 
-definition memory_update_monad:: "(('a::address) memory \<Rightarrow> ('a::address) memory option) \<Rightarrow> 'a expression_monad" where
+definition memory_update_monad:: "(('a::address valtype) memory \<Rightarrow> ('a::address valtype) memory option) \<Rightarrow> 'a expression_monad" where
   "memory_update_monad = my_update_monad state.Memory Memory_update"
 
-definition calldata_update_monad where
-  "calldata_update_monad xs is cd p = option Err (\<lambda>s. state.Calldata s $$ p \<bind> updateCalldata (xs @ is) cd) \<bind> modify \<circ> (calldata_update p) \<bind> K (return Empty)"
+context Contract
+begin
 
-definition (in Contract) storage_update_monad where
+definition storage_update:: "id \<Rightarrow> ('a::address valtype) storage_data \<Rightarrow> ('a::address) state \<Rightarrow> ('a::address) state" where
+  "storage_update i d s = s\<lparr>Storage := (state.Storage s) (this := (state.Storage s this) (i := d))\<rparr>"
+
+definition storage_update_monad where
   "storage_update_monad xs is sd p = option Err (\<lambda>s. updateStore (xs @ is) sd (state.Storage s this p)) \<bind> modify \<circ> (storage_update p) \<bind> K (return Empty)"
 
-fun push where
-  "push d (sdata.Array xs) = Some (sdata.Array (xs @@ d))"
-| "push _ _ = None"
-
-definition (in Contract) allocate::"id \<Rightarrow> ('a::address) expression_monad list \<Rightarrow> ('a::address) sdata \<Rightarrow> ('a::address) expression_monad" where
-  "allocate i es d =
-    do {
-      is \<leftarrow> lfold es;
-      ar \<leftarrow> option Err (\<lambda>s. slookup is (state.Storage s this i) \<bind> push d);
-      storage_update_monad [] is (K ar) i
-    }"
-
-definition stack_check where
-  "stack_check i kf mf cf sf =
-    do {
-      k \<leftarrow> applyf Stack;
-      case k $$ i of
-        Some x \<Rightarrow> case_kdata sf mf cf kf x
-      | None \<Rightarrow> throw Err
-    }"
+end
 
 definition option_check where
   "option_check f m = option Err f \<bind> m"
 
-definition(in Contract) stackLookup::"id \<Rightarrow> ('a::address) expression_monad list \<Rightarrow> ('a::address) expression_monad" where
-  "stackLookup i es =
-    do {
-      is \<leftarrow> lfold es;
-      stack_check i
-        (\<lambda>k. return (Value k))
-        (\<lambda>p. do {
-          (l, md) \<leftarrow> option Err (\<lambda>s. mlookup (state.Memory s) is p);
-          if mdata.is_Value md then return (rvalue.Value (mdata.vt md)) else return (rvalue.Memory l)
-        })
-        (\<lambda>p xs. do {
-          sd \<leftarrow> option Err (\<lambda>s. state.Calldata s $$ p \<bind> clookup (xs@is));
-          if cdata.is_Value sd then return (rvalue.Value (cdata.vt sd)) else return (rvalue.Calldata p (xs@is))
-        })
-        (\<lambda>p xs. do {
-          sd \<leftarrow> option Err (\<lambda>s. slookup (xs@is) (state.Storage s this p));
-          if sdata.is_Value sd then return (rvalue.Value (sdata.vt sd)) else return (rvalue.Storage p (xs@is))
-        })
-    }"
-
-definition(in Contract) arrayLength::"id \<Rightarrow> ('a::address) expression_monad list \<Rightarrow> ('a::address) expression_monad" where
-  "arrayLength i es =
-    do {
-      is \<leftarrow> lfold es;
-      stack_check i
-        (K (throw Err))
-        (\<lambda>p. do {
-          (l, md) \<leftarrow> option Err (\<lambda>s. mlookup (state.Memory s) is p);
-          if mdata.is_Array md then return (rvalue.Value (Sint (of_nat (length (mdata.ar md))))) else throw Err
-        })
-        (\<lambda>p xs. do {
-          sd \<leftarrow> option Err (\<lambda>s. state.Calldata s $$ p \<bind> clookup (xs@is));
-          if cdata.is_Array sd then return (rvalue.Value (Sint (of_nat (length (cdata.ar sd))))) else throw Err
-        })
-        (\<lambda>p xs. do {
-          sd \<leftarrow> option Err (\<lambda>s. slookup (xs@is) (state.Storage s this p));
-          if sdata.is_Array sd then return (rvalue.Value (Sint (of_nat (length (sdata.ar sd))))) else throw Err
-        })
-    }"
-
-subsection \<open>Stack\<close>
-
-primrec (in Contract) assign_stack:: "id \<Rightarrow> ('a::address) valtype list \<Rightarrow> ('a::address) rvalue \<Rightarrow> ('a::address) expression_monad" where
+fun (in Contract) assign_stack::
+  "id \<Rightarrow> ('a::address) valtype list \<Rightarrow> ('a::address) rvalue \<Rightarrow> ('a::address) expression_monad"
+where
   "assign_stack i is (rvalue.Value v) =
     stack_check i
-      (K ((modify (stack_update i (kdata.Value v))) \<bind> K (return Empty)))
-      (\<lambda>p. (memory_update_monad (mvalue_update is p v)))
+      (K (modify (stack_update i (kdata.Value v)) \<bind> K (return Empty)))
+      (\<lambda>l. (memory_update_monad (\<lambda>m. mupdate is (l, (mdata.Value v), m))))
       (K (K (throw Err)))
-      (\<lambda>p xs. storage_update_monad xs is (K (sdata.Value v)) p)"
-| "assign_stack i is (rvalue.Memory p) =
+      (throw Err)
+      (\<lambda>l xs. storage_update_monad xs is (K (storage_data.Value v)) l)
+      (throw Err)"
+| "assign_stack i is (rvalue.Memory l) =
     stack_check i
       (K (throw Err))
-      (\<lambda>p'. case_list is
-        (modify (stack_update i (kdata.Memory p))\<bind> K (return Empty))
-        (K (K (memory_update_monad (marray_update is p' p)))))
+      (\<lambda>l'. case_list is
+        (modify (stack_update i (kdata.Memory l))\<bind> K (return Empty))
+        (K (K (memory_update_monad (\<lambda>m. (m$l) \<bind> (\<lambda>v. mupdate is (l', v, m)))))))
       (K (K (throw Err)))
-      (\<lambda>p' xs. option_check
-        (\<lambda>s. copy_memory_storage (state.Memory s) p)
-        (\<lambda>sd. storage_update_monad xs is (K sd) p'))"
-| "assign_stack i is (rvalue.Calldata p xs) =
+      (throw Err)
+      (\<lambda>l' xs. option_check
+        (\<lambda>s. copy_memory_storage (state.Memory s) l)
+        (\<lambda>sd. storage_update_monad xs is (K sd) l'))
+      (throw Err)"
+| "assign_stack i is (rvalue.Calldata (Some p)) =
     stack_check i
       (K (throw Err))
-      (\<lambda>p'. option_check
-        (\<lambda>s. state.Calldata s $$ p \<bind> clookup (xs @ is))
-        (\<lambda>cd. memory_update_monad (copy_calldata_memory (cd, p'))))
+      (\<lambda>l. option_check
+        (\<lambda>s. state.Calldata s $$ (Location p) \<bind> clookup (Offset p))
+        (\<lambda>cd. memory_update_monad (mupdate is \<circ> (copy_calldata_memory cd l))))
       (K (K (throw Err)))
-      (\<lambda>p' xs'. option_check
-        (\<lambda>s. state.Calldata s $$ p \<bind> clookup (xs @ is))
-        (\<lambda>cd. storage_update_monad xs' is (K (copy_calldata_storage cd)) p'))"
-| "assign_stack i is (rvalue.Storage p xs) =
+      (modify (stack_update i (kdata.Calldata (Some p))) \<bind> K (return Empty))
+      (\<lambda>l xs. option_check
+        (\<lambda>s. state.Calldata s $$ (Location p) \<bind> clookup (Offset p @ is))
+        (\<lambda>cd. storage_update_monad xs is (K (copy_calldata_storage cd)) l))
+      (throw Err)"
+| "assign_stack i is (rvalue.Calldata None) = throw Err"
+| "assign_stack i is (rvalue.Storage (Some p)) =
     stack_check i
       (K (throw Err))
-      (\<lambda>p'. option_check
-        (\<lambda>s. slookup (xs @ is) (state.Storage s this p))
-        (\<lambda>sd. memory_update_monad (copy_storage_memory (sd, p'))))
+      (\<lambda>l. option_check
+        (\<lambda>s. slookup (Offset p) (state.Storage s this (Location p)))
+        (\<lambda>sd. memory_update_monad
+          (\<lambda>m. copy_storage_memory sd l m \<bind>
+            mupdate is)))
       (K (K (throw Err)))
-      (\<lambda>p' xs'. case_list is
-        (modify (stack_update i (kdata.Storage p xs)) \<bind> K (return Empty))
+      (throw Err)
+      (\<lambda>l xs. case_list is
+        (modify (stack_update i (kdata.Storage (Some p))) \<bind> K (return Empty))
         (K (K (option_check
-          (\<lambda>s. slookup (xs @ is) (state.Storage s this p))
-          (\<lambda>sd. storage_update_monad xs' [] (K sd) p')))))"
+          (\<lambda>s. slookup (Offset p @ is) (state.Storage s this (Location p)))
+          (\<lambda>sd. storage_update_monad xs [] (K sd) l)))))
+      (modify (stack_update i (kdata.Storage (Some p))) \<bind> K (return Empty))"
+| "assign_stack i is (rvalue.Storage None) = throw Err"
 | "assign_stack i is rvalue.Empty = throw Err"
 
-definition (in Contract) assign_stack_monad::"String.literal \<Rightarrow> ('a rvalue, ex, 'a state) state_monad list \<Rightarrow> ('a rvalue, ex, 'a state) state_monad \<Rightarrow> ('a rvalue, ex, 'a state) state_monad" where
+definition (in Contract) assign_stack_monad::
+  "String.literal \<Rightarrow> ('a rvalue, ex, 'a state) state_monad list \<Rightarrow> ('a rvalue, ex, 'a state) state_monad \<Rightarrow> ('a rvalue, ex, 'a state) state_monad"
+  ("(_ _ ::= _)" [1000, 61, 0] 61)
+where
   "assign_stack_monad i es m \<equiv> 
     do {
       val \<leftarrow> m;
@@ -461,25 +584,31 @@ definition (in Contract) assign_stack_monad::"String.literal \<Rightarrow> ('a r
       return Empty
     }"
 
-subsection \<open>Storage\<close>
+section \<open>Storage Assignment\<close>
 
-primrec (in Contract) assign_storage:: "id \<Rightarrow> ('a::address) valtype list \<Rightarrow> ('a::address) rvalue \<Rightarrow> ('a::address) expression_monad" where
-  "assign_storage i is (rvalue.Value v) = storage_update_monad [] is (K (sdata.Value v)) i"
-| "assign_storage i is (rvalue.Memory p) =
+fun (in Contract) assign_storage::
+  "id \<Rightarrow> ('a::address) valtype list \<Rightarrow> ('a::address) rvalue \<Rightarrow> ('a::address) expression_monad"
+where
+  "assign_storage i is (rvalue.Value v) = storage_update_monad [] is (K (storage_data.Value v)) i"
+| "assign_storage i is (rvalue.Memory l) =
     (option_check
-      (\<lambda>s. copy_memory_storage (state.Memory s) p)
+      (\<lambda>s. copy_memory_storage (state.Memory s) l)
       (\<lambda>sd. storage_update_monad [] is (K sd) i))"
-| "assign_storage i is (rvalue.Calldata p xs) =
+| "assign_storage i is (rvalue.Calldata (Some p)) =
     (option_check
-      (\<lambda>s. state.Calldata s $$ p \<bind> clookup xs)
+      (\<lambda>s. state.Calldata s $$ (Location p) \<bind> clookup (Offset p))
       (\<lambda>cd. storage_update_monad [] is (K (copy_calldata_storage cd)) i))"
-| "assign_storage i is (rvalue.Storage p xs) =
+| "assign_storage i is (rvalue.Calldata None) = throw Err"
+| "assign_storage i is (rvalue.Storage (Some p)) =
     (option_check
-      (\<lambda>s. slookup xs (state.Storage s this p))
+      (\<lambda>s. slookup (Offset p) (state.Storage s this (Location p)))
       (\<lambda>sd. storage_update_monad [] is (K sd) i))"
+| "assign_storage i is (rvalue.Storage None) = throw Err"
 | "assign_storage i is rvalue.Empty = throw Err"
 
-definition (in Contract) assign_storage_monad where
+definition (in Contract) assign_storage_monad
+("(_ _ ::=\<^sub>s _)" [61, 62, 61] 60)
+  where
   "assign_storage_monad i es m \<equiv> 
     do {
       val \<leftarrow> m;
@@ -510,58 +639,6 @@ definition (in Contract) assign_storage_monad where
       }
   }
 *)
-
-section \<open>Declarations\<close>
-
-definition (in Contract) initStorage::"id \<Rightarrow> ('a::address) sdata \<Rightarrow> ('a::address) expression_monad" where
-  "initStorage i v \<equiv> modify (\<lambda>s. storage_update i v s) \<bind> K (return Empty)"
-
-abbreviation emptyStack::"('a::address) expression_monad" where
-  "emptyStack \<equiv> (modify (Stack_update (K fmempty)) \<bind> K (return Empty))"
-
-definition init::"id \<Rightarrow> ('a::address) valtype \<Rightarrow> ('a::address) expression_monad" where
-  "init i v \<equiv> modify (stack_update i (kdata.Value v)) \<bind> K (return Empty)"
-
-definition minit::"id \<Rightarrow> ('a::address) cdata \<Rightarrow> ('a::address) expression_monad" where
-  "minit i c \<equiv> update (\<lambda>s. let (l,m) = State.minit c (state.Memory s) in (Empty, s\<lparr>Stack := fmupd i (kdata.Memory l) (Stack s), Memory := m\<rparr>))"
-
-definition cinit::"id \<Rightarrow> ('a::address) cdata \<Rightarrow> ('a::address) expression_monad" where
-  "cinit i c \<equiv> modify (calldata_update i c \<circ> stack_update i (kdata.Calldata i [])) \<bind> K (return Empty)"
-
-definition cdecl::"id \<Rightarrow> id \<Rightarrow> ('a::address) valtype list \<Rightarrow> ('a::address) expression_monad" where
-  "cdecl i i' v \<equiv> modify (stack_update i (kdata.Calldata i' v)) \<bind> K (return Empty)"
-
-definition sinit::"id \<Rightarrow> id \<Rightarrow> ('a::address) valtype list \<Rightarrow> ('a::address) expression_monad" where
-  "sinit i i' v \<equiv> modify (stack_update i (kdata.Storage i' v)) \<bind> K (return Empty)"
-
-definition create_memory_value :: "('a::address) valtype \<Rightarrow> (location, unit, ('a::address) memory) state_monad" where
-  "create_memory_value v = 
-    do {
-      pos \<leftarrow> applyf length;
-      modify (\<lambda>m. m @@ mdata.Value v);
-      return pos
-    }"
-
-definition create_memory_array :: "nat \<Rightarrow> (location, unit, ('a::address) memory) state_monad \<Rightarrow> (location, unit, ('a::address) memory) state_monad" where
-  "create_memory_array x mm = 
-    do {
-      ls \<leftarrow> mfold mm x;
-      pos \<leftarrow> applyf length;
-      modify (\<lambda>m. m @@ mdata.Array ls);
-      return pos
-    }"
-
-lemma "P (execute (create_memory_array 2 (create_memory_array 3 (create_memory_value (Bool False)))) [])=
-       P (Normal (8, [mdata.Value (Bool False), mdata.Value (Bool False), mdata.Value (Bool False), mdata.Array [0, 1, 2], mdata.Value (Bool False),
-          mdata.Value (Bool False), mdata.Value (Bool False), mdata.Array [4, 5, 6], mdata.Array [3, 7]]))"
-  by normalization
-
-definition decl_memory_array :: "(location, unit, ('a::address) memory) state_monad \<Rightarrow> ('a::address) expression_monad" where
-  "decl_memory_array mm = create (\<lambda>s.
-    case (execute mm (state.Memory s)) of
-      Normal (pos, m) \<Rightarrow> Normal (rvalue.Memory pos, s\<lparr>Memory := m\<rparr>)
-    | Exception ((),m) \<Rightarrow> Exception (Err,s\<lparr>Memory := m\<rparr>)
-    | NT \<Rightarrow> NT)"
 
 section \<open>Loops\<close>
 
@@ -615,8 +692,6 @@ next
     by (rule Partial_Function.if_mono[OF assms(2)], rule Partial_Function.if_mono[OF assms(3)]) (rule throw_monad_mono) 
 qed
 
-subsection \<open>The While Monad\<close>
-
 partial_function (sm) while_monad :: "('a::address) expression_monad \<Rightarrow> ('a::address) expression_monad \<Rightarrow> ('a::address) expression_monad" where
   "while_monad c m = cond_monad c (bind m (K (while_monad c m))) (return Empty)"
 
@@ -627,13 +702,39 @@ text \<open>
   \<^item> An induction rule for partial correctness @{thm while_monad.raw_induct}
 \<close>
 
-subsection \<open>Require/Assert\<close>
+section \<open>Internal Method Calls\<close>
 
-definition assert_monad :: "('a::address) expression_monad \<Rightarrow> ('a::address) expression_monad" where
- "assert_monad bm = 
-    cond_monad bm (return Empty) (throw Err)"
+definition icall where
+"icall m = 
+do {
+  x \<leftarrow> applyf Stack;
+  r \<leftarrow> m;
+  modify (Stack_update (K x));
+  return r
+}"
 
-section \<open>Solidity Constants\<close>
+lemma icall_mono[mono]:
+  assumes "mono_sm (\<lambda>x. m x)"
+  shows "mono_sm (\<lambda>x. icall (m x))"
+  unfolding icall_def using assms by (simp add:mono)
+
+section \<open>External Method Calls\<close>
+
+definition ecall where
+"ecall m = 
+do {
+  s \<leftarrow> get;
+  r \<leftarrow> m;
+  modify (\<lambda>s'. s'\<lparr>Stack := state.Stack s, Memory := state.Memory s, Calldata := state.Calldata s\<rparr>);
+  return r
+}"
+
+lemma ecall_mono[mono]:
+  assumes "mono_sm (\<lambda>x. m x)"
+  shows "mono_sm (\<lambda>x. ecall (m x))"
+  unfolding ecall_def using assms by (simp add:mono)
+
+section \<open>Transfer\<close>
 
 fun readValue:: "('a::address) rvalue \<Rightarrow> ((('a::address) valtype, ex, ('a::address) state) state_monad)" where
   "readValue (rvalue.Value x) = return x"
@@ -644,24 +745,79 @@ fun readAddress:: "('a::address) valtype \<Rightarrow> ((('a::address), ex, ('a:
 | "readAddress _ = throw Err"
 
 fun readSint:: "('a::address) valtype \<Rightarrow> ((256 word, ex, ('a::address) state) state_monad)" where
-  "readSint (Sint x) = return x"
+  "readSint (Uint x) = return x"
 | "readSint _ = throw Err"
 
-locale Fallback = Contract +
-  constrains this :: "'a::address"
-  fixes fallback::"('a::address) \<Rightarrow> ('a::address) expression_monad"
-  assumes fallback_invariant:
-    "\<And>call:: 'a expression_monad.
-      \<And>P E s.
-      \<lbrakk>\<forall>s r. P s \<and> effect call s r \<longrightarrow> inv r P E;
-      P s\<rbrakk>
-      \<Longrightarrow> (\<forall>a r. effect (fallback a) s r
-           \<longrightarrow> inv r (\<lambda>s'. state.Stack s' = state.Stack s \<and> state.Memory s' = state.Memory s \<and> state.Calldata s' = state.Calldata s \<and> P s')
-                     (\<lambda>s'. state.Stack s' = state.Stack s \<and> state.Memory s' = state.Memory s \<and> state.Calldata s' = state.Calldata s \<and> E s'))"
+context Contract
 begin
 
-definition transfer_monad:: "('a::address) expression_monad \<Rightarrow> ('a::address) expression_monad \<Rightarrow> ('a::address) expression_monad" where
-  "transfer_monad am vm = 
+abbreviation balance_update:: "nat \<Rightarrow> ('a::address) state \<Rightarrow> ('a::address) state" where
+  "balance_update \<equiv> balances_update this"
+
+definition inv:: "'a rvalue \<times> ('a::address) state + ex \<times> ('a::address) state \<Rightarrow> (('a::address) state \<Rightarrow> bool) \<Rightarrow> (('a::address) state \<Rightarrow> bool) \<Rightarrow> bool" where
+  "inv r P Q \<equiv> (case r of Inl a \<Rightarrow> P (snd a)
+                        | Inr a \<Rightarrow> Q (snd a))"
+
+definition inv_state:: "((id \<Rightarrow> ('a::address valtype) storage_data) \<times> nat \<Rightarrow> bool) \<Rightarrow> ('a::address) state \<Rightarrow> bool"
+  where "inv_state i s = i (state.Storage s this, state.Balances s this)"
+
+definition post::
+  "('a::address) state \<Rightarrow> 'a rvalue \<times> ('a::address) state + ex \<times> ('a::address) state
+  \<Rightarrow> (('a::address) state \<Rightarrow> ('a::address) rvalue \<Rightarrow> ('a::address) state \<Rightarrow> bool) \<Rightarrow> (('a::address) state \<Rightarrow> bool)
+  \<Rightarrow> bool" where
+  "post s r I_s I_e \<equiv> (case r of Inl a \<Rightarrow> I_s s (fst a) (snd a)
+                               | Inr a \<Rightarrow> I_e (snd a))"
+
+term "post s r (K (K (inv_state i))) e"
+
+(*
+  reduce post2 for "exc x" to post2 for "x"
+*)
+lemma post_exc_true:
+  assumes "effect (exc x) s r"
+      and "\<And>r. effect x s r \<Longrightarrow> post s r I (K True)"
+    shows "post s r I (K True)"
+  using assms(1) unfolding post_def effect_def exc_def
+  apply (auto simp add:execute_simps) using assms(2) unfolding effect_def post_def
+  by (smt (z3) case_prod_beta ex.case ex.exhaust fst_def is_Normal_def old.sum.simps(5) prod.collapse result.case_eq_if result.disc(2) result.disc(3) result.distinct_disc(1) result.sel(1) snd_def)
+
+lemma post_exc_false:
+  assumes "effect (exc x) s r"
+      and "\<And>r. effect x s r \<Longrightarrow> post s r I (K False)"
+    shows "post s r I (K False)"
+  using assms(1) unfolding post_def effect_def exc_def
+  apply (auto simp add:execute_simps) using assms(2) unfolding effect_def post_def
+  apply (smt (z3) case_prod_beta ex.case ex.exhaust fst_def is_Normal_def old.sum.simps(5) prod.collapse result.case_eq_if result.disc(2) result.disc(3) result.distinct_disc(1) result.sel(1) snd_def)
+  using assms(2) unfolding effect_def post_def
+  by (metis (no_types, lifting) K.simps case_prod_beta case_sum_o_inj(2) result.case_eq_if result.disc(4)
+      result.distinct_disc(5) surjective_sum)
+
+(*
+  reduce post to post2
+*)
+lemma post_true:
+  assumes "effect (exc x) s r"
+      and "I' s"
+      and "post s r I (K True)"
+    shows "post s r I I'"
+  using assms unfolding post_def effect_def
+  apply (auto simp add: execute_simps)
+  unfolding exc_def apply (simp add:execute_simps)
+  by (metis (mono_tags, lifting) ex.exhaust result.case_eq_if result.disc(4) result.disc(6) result.sel(2) snd_conv split_beta)
+
+end
+
+locale External = Contract +
+  constrains this :: "'a::address"
+  fixes external::"('d \<Rightarrow> 'a expression_monad) \<Rightarrow> ('a::address) expression_monad"
+  assumes external_mono[mono]: "mono_sm (\<lambda>call. external call)"
+begin
+
+definition transfer_monad::
+  "('d \<Rightarrow> 'a expression_monad) \<Rightarrow> ('a::address) expression_monad \<Rightarrow> ('a::address) expression_monad \<Rightarrow> ('a::address) expression_monad"
+("\<langle>transfer\<rangle>")  
+where
+  "transfer_monad call am vm = 
     do {
       ak \<leftarrow> am;
       av \<leftarrow> readValue ak;
@@ -672,33 +828,273 @@ definition transfer_monad:: "('a::address) expression_monad \<Rightarrow> ('a::a
       assert Err (\<lambda>s. Balances s this \<ge> unat v);
       modify (\<lambda>s. balances_update this (Balances s this - unat v) s);
       modify (\<lambda>s. balances_update a (Balances s a + unat v) s);
-      fallback a
+      ecall (external call)
     }"
 
-end
-
-locale Method =
-  fixes msg_sender :: "'a::address" (*address of calling contract*)
-    and msg_value :: "256 word" (*money send*)
-  assumes sender_neq_null: "msg_sender \<noteq> null"
-begin
-
-definition sender_monad where
-  "sender_monad = address_monad msg_sender"
-
-definition value_monad where
-  "value_monad = sint_monad msg_value"
+lemma transfer_mono[mono]:
+  shows "monotone sm.le_fun sm_ord
+     (\<lambda>f. transfer_monad f m n)"
+  unfolding transfer_monad_def
+  by (auto intro!: mono)
 
 end
 
-locale Solidity = Keccak256 + Method + Fallback +
+section \<open>Solidity\<close>
+
+locale Solidity = Keccak256 + Method + External +
   constrains keccak256::"('a::address) rvalue \<Rightarrow> ('a::address) rvalue"
          and msg_sender :: "'a::address"
          and this::"'a::address"
-         and fallback::"('a::address) \<Rightarrow> ('a::address) expression_monad"
+         and external::"('d \<Rightarrow> 'a expression_monad) \<Rightarrow> ('a::address) expression_monad"
 begin
   definition init_balance:: "('a rvalue, ex, ('a::address) state) state_monad" where
     "init_balance = modify (\<lambda>s. balance_update (Balances s this + unat msg_value) s) \<bind> K (return Empty)"
+
+  definition init_balance_np:: "('a rvalue, ex, ('a::address) state) state_monad" where
+    "init_balance_np = modify (\<lambda>s. balance_update (Balances s this) s) \<bind> K (return Empty)"
+
 end
+
+section \<open>Arrays\<close>
+
+definition array where "array i x = replicate i x"
+
+lemma length_array[simp]: "length (array x y) = x"
+  unfolding array_def
+  by simp
+
+
+lemma fold_map_write_replicate_length:
+  assumes "fold_map Memory.write (replicate n (adata.Value v)) m = (x1, x2)"
+    shows "length x1 = n"
+  using assms
+proof (induction n arbitrary: x1 m)
+  case 0
+  then show ?case by simp 
+next
+  case (Suc n)
+  from Suc.prems obtain x1a
+    where *: "fold_map Memory.write (replicate n (adata.Value v)) (m @ [mdata.Value v]) = (x1a, x2)"
+      and **:"x1 = length m # x1a"
+    by (auto simp add: array_def length_append_def split:prod.split_asm)
+  then show ?case
+  proof (cases "n = 0")
+    case True
+    then show ?thesis using Suc.prems(1) by (auto split:prod.split_asm)
+  next
+    case False
+    then show ?thesis using * Suc by (auto simp add: length_append_def)
+  qed
+qed
+
+lemma fold_map_write_replicate_value:
+  assumes "fold_map Memory.write (replicate n (adata.Value (Uint 0))) m = (x1, x2)"
+      and "x < n"
+    shows "x1 ! x < length x2 \<and> (\<exists>ix. x2 ! (x1 ! x) = mdata.Value (Uint ix))"
+  using assms
+proof (induction n arbitrary: x1 m x)
+  case 0
+  then show ?case by simp
+next
+  case (Suc n)
+  from Suc.prems
+    obtain x1a
+      where *: "fold_map Memory.write (replicate n (adata.Value (Uint 0))) (m @ [mdata.Value (Uint 0)]) = (x1a, x2)"
+        and **:"x1 = length m # x1a"
+      by (simp add: length_append_def split:prod.split_asm)
+  then show ?case
+  proof (cases "n = 0")
+    case True
+    then show ?thesis using Suc.prems(1,2) by (auto simp add: length_append_def)
+  next
+    case False
+    then show ?thesis
+    proof (cases "x = 0")
+      case True
+      moreover from False
+        have "(replicate n (adata.Value (Uint 0))) \<noteq> []" by auto
+      then have "sprefix (m @ [mdata.Value (Uint 0)]) x2"
+        using write_fold_map_sprefix[of "(replicate n (adata.Value (Uint 0)))" " (m @ [mdata.Value (Uint 0)])"]
+        unfolding sprefix_def using * by simp
+      ultimately show ?thesis unfolding sprefix_def
+        using ** sprefix_def by (auto simp add: array_def length_append_def split:prod.split_asm)
+   next
+      case _: False
+      moreover have "x1a ! (x - 1) < length x2 \<and> (\<exists>ix. x2 ! (x1a ! (x - 1)) = mdata.Value (Uint ix))"
+        using Suc.IH[OF *] Suc.prems(2) False by simp
+      ultimately show ?thesis
+        using * Suc.prems(1) by (auto simp add: length_append_def)
+    qed
+  qed
+qed
+
+lemma write_array_typing_value:
+  assumes "Memory.write (adata.Array (array (unat si) (adata.Value (Uint 0)))) [] = (x1, x2)"
+    shows "x1<length x2 \<and> (\<exists>ma0. x2 ! x1 = mdata.Array ma0 \<and> (\<forall>i<length ma0. (ma0 ! i) < length x2 \<and> (\<exists>ix. x2 ! (ma0 ! i) = mdata.Value (Uint ix))))"
+proof -
+  from assms obtain x1a x2a
+    where *:"fold_map Memory.write (replicate (unat si) (adata.Value (Uint 0))) [] = (x1a, x2a)"
+      and "x1 = length x2a"
+      and "x2 = x2a @ [mdata.Array x1a]"
+    by (simp add: array_def length_append_def split:prod.split_asm)
+  moreover have "(\<forall>i<length x1a. (x1a ! i) < length x2a \<and> (\<exists>ix. x2 ! (x1a ! i) = mdata.Value (Uint ix)))"
+  proof (rule allI, rule impI)
+    fix i assume "i < length x1a"
+    moreover have "length x1a = unat si" using fold_map_write_replicate_length[OF *] by simp
+    ultimately show "(x1a ! i) < length x2a \<and> (\<exists>ix. x2 ! (x1a ! i) = mdata.Value (Uint ix))"
+      using fold_map_write_replicate_value[OF *, of i]
+      by (simp add: \<open>x2 = x2a @ [mdata.Array x1a]\<close> nth_append_left)
+  qed
+  ultimately show ?thesis by auto
+qed
+
+lemma mupdate_array_typing_value:
+  assumes "state.Memory sa ! ml = mdata.Array ma0"
+      and "\<forall>i<length ma0. (ma0 ! i) < length (state.Memory sa) \<and> (\<exists>ix. state.Memory sa ! (ma0 ! i) = mdata.Value (Uint ix))"
+      and "mupdate [Uint xa] (ml, mdata.Value (Uint x), state.Memory sa) = Some yg"
+    shows "\<exists>ma0. yg ! ml = mdata.Array ma0
+          \<and> (\<forall>i<length ma0. (ma0 ! i) < length yg \<and> (\<exists>ix. yg ! (ma0 ! i) = mdata.Value (Uint ix)))"
+proof -
+  from assms have "ma0 ! unat xa \<noteq> ml"
+  proof -
+    from assms(1,2,3) obtain ix
+      where "(ma0 ! (unat xa)) < length (state.Memory sa)"
+        and "(state.Memory sa ! (ma0 ! (unat xa)) = mdata.Value (Uint ix))"
+      by (auto simp add: case_memory_def nth_safe_def split:if_split_asm)
+    then show ?thesis using assms(1) by auto
+  qed
+  then have "yg ! ml = mdata.Array ma0"
+    using assms(1,3)
+    by (auto simp add: case_memory_def nth_safe_def list_update_safe_def split:if_split_asm)
+  moreover have "\<forall>i<length ma0. (ma0 ! i) < length yg \<and> (\<exists>ix. yg ! (ma0 ! i) = mdata.Value (Uint ix))"
+  proof (rule allI, rule impI)
+    fix i assume "i < length ma0"
+    show "(ma0 ! i) < length yg \<and> (\<exists>ix. yg ! (ma0 ! i) = mdata.Value (Uint ix))"
+    proof (cases "ma0 ! i = ma0 ! unat xa")
+      case True
+      then show ?thesis using assms(1,3) 
+        by (auto simp add: case_memory_def nth_safe_def list_update_safe_def split:if_split_asm)
+    next
+      case False
+      then show ?thesis using \<open>i < length ma0\<close> assms(1,2,3) 
+        by (auto simp add: case_memory_def nth_safe_def list_update_safe_def split:if_split_asm)
+    qed
+  qed
+  ultimately show ?thesis by blast
+qed
+
+section \<open>Declarations\<close>
+(*
+Used in ML code
+*)
+definition (in Contract) initStorage::"id \<Rightarrow> ('a::address valtype) storage_data \<Rightarrow> ('a::address) expression_monad" where
+  "initStorage i v \<equiv> modify (\<lambda>s. storage_update i v s) \<bind> K (return Empty)"
+
+definition kinit::"('a::address valtype) kdata \<Rightarrow> id \<Rightarrow> ('a::address) expression_monad" where
+  "kinit v i \<equiv> modify (stack_update i v) \<bind> K (return Empty)"
+
+definition init::"('a::address) valtype \<Rightarrow> id \<Rightarrow> ('a::address) expression_monad" where
+  "init \<equiv> kinit \<circ> kdata.Value"
+
+definition "write"::"('a::address valtype) adata \<Rightarrow> id \<Rightarrow> ('a::address) expression_monad" where
+  "write c i \<equiv> update (\<lambda>s. let (l,m) = Memory.write c (state.Memory s) in (Empty, s\<lparr>Stack := fmupd i (kdata.Memory l) (Stack s), Memory := m\<rparr>))"
+
+definition cinit::"('a::address valtype) call_data \<Rightarrow> id \<Rightarrow> ('a::address) expression_monad" where
+  "cinit c i \<equiv> modify (calldata_update i c \<circ> stack_update i (kdata.Calldata (Some \<lparr>Location=i,Offset= []\<rparr>))) \<bind> K (return Empty)"
+
+subsection \<open>Stack Variables\<close>
+
+datatype VType =
+  TBool | TSint | TAddress | TBytes nat \<comment> \<open>width should be restricted to [1..32]\<close>
+
+subsection \<open>Default values\<close>
+
+definition mapping where "mapping x = (\<lambda>_. x)"
+
+fun default:: "VType \<Rightarrow> 'a::address valtype" where
+   "default TBool = Bool False"
+ | "default TSint = Uint 0"
+ | "default TAddress = Address null"
+ | "default (TBytes n) = Bytes (array n (CHR 0x00))"
+
+definition decl::"VType \<Rightarrow> id \<Rightarrow> ('a::address) expression_monad"
+where
+  "decl \<equiv> init \<circ> default"
+
+(*
+  This should be used in user code
+*)
+abbreviation decl'::"id \<Rightarrow> VType \<Rightarrow> ('a::address) expression_monad"
+  ("(_ :: _)" [61, 61] 60)
+where
+  "decl' x y \<equiv> decl y x"
+
+subsection \<open>Storage Variables\<close>
+
+datatype SType =
+  TValue VType | TArray nat SType | DArray SType | TMap SType SType | TEnum "SType list"
+
+term "DArray (TValue (TBytes 1))"
+ML \<open>
+val it = \<^term>\<open>DArray (TValue (TBytes 1))\<close>
+\<close>
+
+fun sdefault:: "SType \<Rightarrow> 'a::address valtype storage_data" where
+   "sdefault (TValue t) = storage_data.Value (default t)"
+ | "sdefault (TArray l t) = storage_data.Array (array l (sdefault t))"
+ | "sdefault (DArray t) = storage_data.Array []"
+ | "sdefault (TMap _ t) = storage_data.Map (mapping (sdefault t))"
+ | "sdefault (TEnum xs) = storage_data.Array []"
+
+definition sinit::"id \<Rightarrow> ('a::address) expression_monad" where
+  "sinit i \<equiv> modify (stack_update i (kdata.Storage None)) \<bind> K (return Empty)"
+
+(*
+  This should be used in user code
+*)
+fun sdecl::"SType \<Rightarrow> id \<Rightarrow> ('a::address) expression_monad" where
+   "sdecl (TValue _) = K (throw Err)"
+ | "sdecl _ = sinit"
+declare sdecl.simps[simp del]
+
+fun push where
+  "push d (storage_data.Array xs) = Some (storage_data.Array (xs @@ d))"
+| "push _ _ = None"
+
+definition (in Contract) allocate::"id \<Rightarrow> ('a::address) expression_monad list \<Rightarrow> ('a::address valtype) storage_data \<Rightarrow> ('a::address) expression_monad" where
+  "allocate i es d =
+    do {
+      is \<leftarrow> lfold es;
+      ar \<leftarrow> option Err (\<lambda>s. slookup is (state.Storage s this i) \<bind> push d);
+      storage_update_monad [] is (K ar) i
+    }"
+
+subsection \<open>Calldata Variables\<close>
+
+datatype CType =
+  TValue VType | TArray nat CType | DArray CType | TEnum "CType list"
+
+fun cdefault:: "CType \<Rightarrow> 'a::address valtype adata" where
+   "cdefault (TValue t) = adata.Value (default t)"
+ | "cdefault (TArray l t) = adata.Array (array l (cdefault t))"
+ | "cdefault (DArray t) = adata.Array []"
+ | "cdefault (TEnum xs) = adata.Array []"
+
+subsection \<open>Memory Variables\<close>
+
+(*
+  This should be used in user code
+*)
+definition mdecl::"CType \<Rightarrow> id \<Rightarrow> ('a::address) expression_monad" where
+  "mdecl = write \<circ> cdefault"
+
+definition create_memory_array where
+  "create_memory_array i t sm =
+    do {
+      s \<leftarrow> sm;
+      (case s of
+        rvalue.Value (Uint s') \<Rightarrow> write (adata.Array (array (unat s') (cdefault t))) i
+      | _ \<Rightarrow> throw Err)
+    }"
 
 end
