State.thy
@@ -1,33 +1,30 @@
 theory State
-imports Finite_Map_Extras Utils "HOL-Library.Word"
+imports Stores "HOL-Library.Word"
 begin
 
-section \<open>Value Types\<close>
+section \<open>Value types\<close>
 
-subsection \<open>Definition\<close>
-
-type_synonym bytes = String.literal
+type_synonym bytes = string
 type_synonym id = String.literal
 
 datatype ('a::address) valtype =
   Bool (bool: bool)
-| Sint (sint: "256 word")
-| Address 'a
-| Bytes bytes
+| Uint (uint: "256 word")
+| Address (ad: 'a)
+| Bytes (bytes: bytes) \<comment>\<open>bytes1, ..., bytes32\<close>
 
-subsection \<open>Default values\<close>
+instantiation valtype :: (address) vtype
+begin
 
-definition sint where "sint = Sint 0"
+fun to_nat_valtype::"'a valtype \<Rightarrow> nat option" where
+  "to_nat_valtype (Uint x) = Some (unat x)"
+| "to_nat_valtype _ = None"
 
-definition bytes where "bytes = Bytes (STR ''0000000000000000000000000000000000000000000000000000000000000000'')"
+instance ..
 
-definition address where "address = Address null"
+end
 
-definition bool where "bool = Bool False"
-
-definition mapping where "mapping x = (\<lambda>_. x)"
-
-subsection \<open>Common functions\<close>
+section \<open>Common functions\<close>
 
 fun lift_bool_unary::"(bool \<Rightarrow> bool) \<Rightarrow> ('a::address) valtype \<Rightarrow> ('a::address) valtype option" where
   "lift_bool_unary op (Bool b) = Some (Bool (op b))"
@@ -47,28 +44,28 @@ definition vtor where
   "vtor = lift_bool_binary (\<or>)"
 
 fun vtequals where
-  "vtequals (Sint l) (Sint r) = Some (Bool (l = r))"
+  "vtequals (Uint l) (Uint r) = Some (Bool (l = r))"
 | "vtequals (Address l) (Address r) = Some (Bool (l = r))"
 | "vtequals (Bool l) (Bool r) = Some (Bool (l = r))"
 | "vtequals (Bytes l) (Bytes r) = Some (Bool (l = r))"
 | "vtequals _ _ = None"
 
 fun lift_int_comp::"(256 word \<Rightarrow> 256 word \<Rightarrow> bool) \<Rightarrow> ('a::address) valtype \<Rightarrow> ('a::address) valtype \<Rightarrow> ('a::address) valtype option" where
-  "lift_int_comp op (Sint l) (Sint r) = Some (Bool (op l r))"
+  "lift_int_comp op (Uint l) (Uint r) = Some (Bool (op l r))"
 | "lift_int_comp _ _ _ = None"
 
 definition vtless where
   "vtless = lift_int_comp (<)"
 
 fun lift_int_binary::"(256 word \<Rightarrow> 256 word \<Rightarrow> 256 word) \<Rightarrow> ('a::address) valtype \<Rightarrow> ('a::address) valtype \<Rightarrow> ('a::address) valtype option" where
-  "lift_int_binary op (Sint l) (Sint r) = Some (Sint (op l r))"
+  "lift_int_binary op (Uint l) (Uint r) = Some (Uint (op l r))"
 | "lift_int_binary _ _ _ = None"
 
 definition vtplus where
   "vtplus = lift_int_binary (+)"
 
 fun vtplus_safe::"('a::address) valtype \<Rightarrow> ('a::address) valtype \<Rightarrow> ('a::address) valtype option" where
-  "vtplus_safe (Sint l) (Sint r) = (if unat l + unat r < 2^256 then Some (Sint (l + r)) else None)"
+  "vtplus_safe (Uint l) (Uint r) = (if unat l + unat r < 2^256 then Some (Uint (l + r)) else None)"
 | "vtplus_safe _ _ = None"
 
 declare vtplus_safe.simps[simp del]
@@ -77,7 +74,7 @@ definition vtminus where
   "vtminus = lift_int_binary (-)"
 
 fun vtminus_safe::"('a::address) valtype \<Rightarrow> ('a::address) valtype \<Rightarrow> ('a::address) valtype option" where
-  "vtminus_safe (Sint l) (Sint r) = (if r \<le> l then Some (Sint (l - r)) else None)"
+  "vtminus_safe (Uint l) (Uint r) = (if r \<le> l then Some (Uint (l - r)) else None)"
 | "vtminus_safe _ _ = None"
 
 declare vtminus_safe.simps[simp del]
@@ -85,350 +82,87 @@ declare vtminus_safe.simps[simp del]
 definition vtmult where
   "vtmult = lift_int_binary (*)"
 
+fun vtmult_safe::"('a::address) valtype \<Rightarrow> ('a::address) valtype \<Rightarrow> ('a::address) valtype option" where
+  "vtmult_safe (Uint l) (Uint r) = (if unat l * unat r < 2^256 then Some (Uint (l * r)) else None)"
+| "vtmult_safe _ _ = None"
+
+declare vtmult_safe.simps[simp del]
+
 definition vtmod where
   "vtmod = lift_int_binary (mod)"
 
-subsection \<open>Examples\<close>
+section \<open>Operations on bytes\<close>
 
-definition "vt_true = Bool True"
-definition "vt_false = Bool False"
-definition "vt_sint_m10 = Sint (-10)"
-definition "vt_sint_1 = Sint 1"
-definition "vt_sint_2 = Sint 2"
-definition "vt_sint_10 = Sint 10"
-definition "vt_address = Address null"
+(* indexing bytes_n returns bytes_1 *)
+fun vtbytes_index :: "('a::address) valtype \<Rightarrow> ('a::address) valtype \<Rightarrow> ('a::address) valtype option" where
+  "vtbytes_index (Bytes xs) (Uint i) = (if unat i < length xs then Some (Bytes [xs ! unat i]) else None)"
+| "vtbytes_index _ _ = None"
 
-section \<open>Storage\<close>
+definition zipWith :: "('a \<Rightarrow> 'b \<Rightarrow> 'c) \<Rightarrow> 'a list \<Rightarrow> 'b list \<Rightarrow> 'c list" where
+  "zipWith op xs ys = map (\<lambda> (x, y). op x y) (zip xs ys)"
 
-subsection \<open>Definition\<close>
+fun lift_bytes_binary::"(char \<Rightarrow> char \<Rightarrow> char) \<Rightarrow> ('a::address) valtype \<Rightarrow> ('a::address) valtype \<Rightarrow> ('a::address) valtype option" where
+  "lift_bytes_binary op (Bytes l) (Bytes r) = (if length l = length r then Some (Bytes (zipWith op l r)) else None)"
+| "lift_bytes_binary _ _ _ = None"
 
-subsubsection \<open>Definition\<close>
+fun lift_bytes_unary::"(char \<Rightarrow> char) \<Rightarrow> ('a::address) valtype \<Rightarrow> ('a::address) valtype option" where
+  "lift_bytes_unary op (Bytes l) = Some (Bytes (map op l))"
+| "lift_bytes_unary _ _ = None"
 
-datatype ('a::address) sdata =
-  is_Value: Value (vt:"('a::address) valtype")
-| is_Array: Array (ar: "('a::address) sdata list")
-| is_Map: Map (mp: "('a::address) valtype \<Rightarrow> ('a::address) sdata")
+definition word8_to_char :: "8 word \<Rightarrow> char" where
+  "word8_to_char w = char_of (unat w)"
 
-abbreviation storage_check where "storage_check sd vf af mf \<equiv> case_sdata vf af mf sd"
+definition char_to_word8 :: "char \<Rightarrow> 8 word" where
+  "char_to_word8 c = of_nat (of_char c)"
 
-subsubsection \<open>Examples\<close>
+definition op_word8_to_char :: "(8 word \<Rightarrow> 8 word \<Rightarrow> 8 word) \<Rightarrow> (char \<Rightarrow> char \<Rightarrow> char)" where
+  "op_word8_to_char op x y = word8_to_char (op (char_to_word8 x) (char_to_word8 y))"
 
-definition "sd_true = Value vt_true"
-definition "sd_false = Value vt_false"
-definition "sd_sint8_m10 = Value vt_sint_m10"
-definition "sd_uint8_10 = Value vt_sint_10"
-definition "sd_address = Value vt_address"
-definition "(sd_Array_3_true::aspace sdata) = Array [sd_true,sd_true,sd_true]"
-definition "(sd_Array_3_false::aspace sdata) = Array [sd_false,sd_false,sd_false]"
-definition "(sd_Array_2_3_true_false::aspace sdata) = Array [sd_Array_3_true, sd_Array_3_false]"
-definition "(sd_Array_2_3_false_false::aspace sdata) = Array [sd_Array_3_false, sd_Array_3_false]"
+context
+  includes bit_operations_syntax
+begin
 
-subsection \<open>Lookup\<close>
+definition vtbytes_and where
+  "vtbytes_and = lift_bytes_binary (op_word8_to_char (AND))"
 
-subsubsection \<open>Definition\<close>
+definition vtbytes_or where
+  "vtbytes_or = lift_bytes_binary (op_word8_to_char (OR))"
 
-text \<open>
-  slookup is sd navigates storage sd according to the index sequence is.
-\<close>
-fun slookup :: "('a::address) valtype list \<Rightarrow> ('a::address) sdata \<Rightarrow> ('a::address) sdata option" where
-  "slookup [] s = Some s"
-| "slookup (valtype.Sint i # is) (sdata.Array xs) = xs $ unat i \<bind> slookup is"
-| "slookup (i # is) (Map f) = slookup is (f i)"
-| "slookup _ _ = None"
+definition vtbytes_xor where
+  "vtbytes_xor = lift_bytes_binary (op_word8_to_char (XOR))"
 
-subsubsection \<open>Examples\<close>
+definition vtbytes_not where
+  "vtbytes_not = lift_bytes_unary (\<lambda> x. word8_to_char ((NOT) (char_to_word8 x)))"
 
-lemma "P (slookup [vt_sint_1, vt_sint_2::aspace valtype] sd_Array_2_3_true_false) = P (Some (Value (Bool False)))"
-  by normalization
+end
 
-subsection \<open>Update\<close>
+fun resize_list :: "nat \<Rightarrow> 'a \<Rightarrow> 'a list \<Rightarrow> 'a list" where
+  "resize_list m pad xs =
+     (if length xs < m
+      then xs @ replicate (m - length xs) pad
+      else take m xs)"
 
-subsubsection \<open>Definition\<close>
-
-fun updateStore :: "('a::address) valtype list \<Rightarrow> (('a::address) sdata \<Rightarrow> ('a::address) sdata) \<Rightarrow> ('a::address) sdata \<Rightarrow> ('a::address) sdata option" where
-  "updateStore [] f v = Some (f v)"
-| "updateStore (valtype.Sint i # is) f (sdata.Array xs) = xs $ (unat i) \<bind> updateStore is f \<bind> list_update_safe xs (unat i) \<bind> Some \<circ> sdata.Array"
-| "updateStore (i # is) f (Map m) = updateStore is f (m i) \<bind> Some \<circ> sdata.Map \<circ> fun_upd m i"
-| "updateStore _ _ _ = None"
-
-subsubsection \<open>Examples\<close>
-
-lemma "P (updateStore [vt_sint_1,vt_sint_2] (K sd_true) sd_Array_2_3_true_false)
-  = P (Some (Array [Array [Value (Bool True), Value (Bool True), Value (Bool True)], Array [Value (Bool False), Value (Bool False), Value (Bool True)]]))"
-  by normalization
-
-section \<open>Memory\<close>
-
-subsection \<open>Definition\<close>
-
-subsubsection \<open>Definition\<close>
-
-type_synonym location = nat
-
-datatype ('a::address) mdata =
-  is_Value: Value (vt: "('a::address) valtype")
-| is_Array: Array (ar: "location list")
-
-definition case_memory where
-  "case_memory m l vf af \<equiv>
-    (case m$l of
-      Some (mdata.Value v) \<Rightarrow> vf v
-    | Some (mdata.Array xs) \<Rightarrow> af xs
-    | None \<Rightarrow> None)"
-
-lemma case_memory_cong[fundef_cong]:
-  assumes "\<And>v. m$l = Some (mdata.Value v) \<Longrightarrow> vf1 v = vf2 v"
-      and "\<And>xs. m$l = Some (mdata.Array xs) \<Longrightarrow> af1 xs = af2 xs"
-    shows "case_memory m l vf1 af1 = case_memory m l vf2 af2"
-  unfolding case_memory_def using assms by (simp split: option.split mdata.split) 
-
-subsubsection \<open>Examples\<close>
-
-definition "md_true = Value vt_true"
-definition "md_false = Value vt_false"
-definition "md_sint_m10 = Value vt_sint_m10"
-definition "md_uint_10 = Value vt_sint_10"
-definition "md_address = Value vt_address"
-
-type_synonym 'a memory = "'a mdata list"
-definition "mem_Array_2_3_true_false = [md_true,md_true,md_true,Array [0,1,2],md_false,md_false,md_false,Array [4,5,6],Array [3,7]]"
-definition "mem_Array_2_3_false_false = [md_false,md_false,md_false,Array [0,1,2],md_false,md_false,md_false,Array [4,5,6],Array [3,7]]"
-definition "mem_sint_m10_uint_10= [md_sint_m10,md_uint_10]"
-
-subsection \<open>Lookup\<close>
-
-subsubsection \<open>Definition\<close>
-
-fun marray_lookup :: "('a::address) memory \<Rightarrow> ('a::address) valtype list \<Rightarrow> location \<Rightarrow> (location \<times> location list \<times> nat) option" where
-  "marray_lookup _ [] _  = None"
-| "marray_lookup m [Sint i] l =
-    case_memory m l
-      (K None)
-      (\<lambda>xs. Some (l, xs, unat i))"
-| "marray_lookup m (Sint i # is) l =
-    case_memory m l
-      (K None)
-      (\<lambda>xs. xs $ unat i \<bind> marray_lookup m is)"
-| "marray_lookup _ _ _ = None"
-
-fun mlookup :: "('a::address) memory \<Rightarrow> ('a::address) valtype list \<Rightarrow> location \<Rightarrow> (location \<times> ('a::address) mdata) option" where
-  "mlookup m [] l = m $ l \<bind> (\<lambda>v. Some (l,v))"
-| "mlookup m xs l = marray_lookup m xs l \<bind> (\<lambda>(_, xs', i). nth_safe m (xs'!i) \<bind> (\<lambda>v. Some (xs'!i,v)))"
-
-fun update::"('a::address) memory \<Rightarrow> location \<Rightarrow> (location \<times> location list \<times> nat) \<Rightarrow> ('a::address) memory" where
-"update m l' (l, ls, n) = m[l:=mdata.Array (ls[n:=l'])]"
-
-fun marray_update :: "('a::address) valtype list \<Rightarrow> location \<Rightarrow> location \<Rightarrow> ('a::address) memory \<Rightarrow> ('a::address) memory option" where
-  "marray_update xs l l' m = marray_lookup m xs l \<bind> Some \<circ> update m l'"
-
-fun mvalue_update :: "('a::address) valtype list \<Rightarrow> location \<Rightarrow> ('a::address) valtype \<Rightarrow> ('a::address) memory \<Rightarrow> ('a::address) memory option" where
-  "mvalue_update xs l v m = marray_lookup m xs l \<bind> (\<lambda>(x, ls, i). ls$i \<bind> (\<lambda>i'. Some (list_update m i' (mdata.Value v))))"
-
-subsubsection \<open>Examples\<close>
-
-lemma "mlookup mem_Array_2_3_true_false [Sint 1, Sint 2] 8 = Some (6, mdata.Value (Bool False))" by normalization
-
-lemma "mlookup mem_Array_2_3_true_false [Sint 0] 8 = Some (3, mdata.Array [0, 1, 2])" by normalization
-
-lemma "marray_update [Sint 1, Sint 2] 8 2 mem_Array_2_3_true_false = Some (mem_Array_2_3_true_false[7:=mdata.Array [4, 5, 2]])" by normalization
-
-section \<open>Calldata\<close>
-
-subsection \<open>Definition\<close>
-
-subsubsection \<open>Definition\<close>
-
-datatype ('a::address) cdata =
-  is_Value: Value (vt: "('a::address) valtype")
-| is_Array: Array (ar: "('a::address) cdata list")
-
-abbreviation case_cdata where "case_cdata cd vf af \<equiv> cdata.case_cdata vf af cd"
-
-subsubsection \<open>Examples\<close>
-
-definition "cd_true = Value vt_true"
-definition "cd_false = Value vt_false"
-definition "cd_sint8_m10 = Value vt_sint_m10"
-definition "cd_uint8_10 = Value vt_sint_10"
-definition "cd_address = Value vt_address"
-definition "cd_Array_3_true = Array [cd_true,cd_true,cd_true]"
-definition "cd_Array_3_false = Array [cd_false,cd_false,cd_false]"
-definition "cd_Array_2_3_true_false = Array [cd_Array_3_true, cd_Array_3_false]"
-definition "cd_Array_2_3_false_false = Array [cd_Array_3_false, cd_Array_3_false]"
-
-subsection \<open>Lookup\<close>
-
-subsubsection \<open>Definition\<close>
-
-text \<open>
-  clookup is cd navigates calldata cd according to the index sequence is.
-\<close>
-fun clookup :: "('a::address) valtype list \<Rightarrow> ('a::address) cdata \<Rightarrow> ('a::address) cdata option" where
-  "clookup [] s = Some s"
-| "clookup (valtype.Sint i # is) (cdata.Array xs) = xs $ unat i \<bind> clookup is"
-| "clookup _ _ = None"
-
-subsubsection \<open>Examples\<close>
-
-lemma "clookup [vt_sint_1, vt_sint_2] cd_Array_2_3_true_false = Some (cdata.Value (Bool False))" by normalization
-
-subsection \<open>Update\<close>
-
-subsubsection \<open>Definition\<close>
-
-fun updateCalldata :: "('a::address) valtype list \<Rightarrow> ('a::address) cdata \<Rightarrow> ('a::address) cdata \<Rightarrow> ('a::address) cdata option" where
-  "updateCalldata [] v _ = Some v"
-| "updateCalldata (valtype.Sint i # is) v (cdata.Array xs) = (xs $ (unat i) \<bind> updateCalldata is v) \<bind> Some \<circ> cdata.Array \<circ> list_update xs (unat i)"
-| "updateCalldata _ _ _ = None"
-
-subsubsection \<open>Examples\<close>
-
-lemma "updateCalldata [vt_sint_1, vt_sint_2::aspace valtype] cd_true cd_Array_2_3_true_false =
-  Some (cdata.Array [cd_Array_3_true, cdata.Array [cd_false, cd_false, cd_true]])"
-  by (normalization)
-
-section \<open>Initialize Memory\<close>
-
-function minit :: "('a::address) cdata \<Rightarrow> ('a::address) memory \<Rightarrow> nat \<times> ('a::address) memory" where
-  "minit (cdata.Value x) m = length_append m (mdata.Value x)"
-| "minit (cdata.Array ds) m = (let (ns, m') = fold_map minit ds m in (length_append m' (mdata.Array ns)))"
-  by pat_completeness auto
-termination
-  apply (relation "measure (\<lambda>(s,b). size (s))") apply auto
-  by (meson Suc_n_not_le_n leI size_list_estimation')
-
-lemma "minit (cdata.Array [cdata.Value (Sint 0), cdata.Value (Sint 0), cdata.Value (Sint 0)]) ([]::aspace mdata list)
-      = (3, [mdata.Value (Sint 0), mdata.Value (Sint 0), mdata.Value (Sint 0), mdata.Array [0, 1, 2]])"
-  by eval
-
-section \<open>Copy Between Stores\<close>
-
-subsection \<open>Termination Lemmas\<close>
-
-lemma card_less_card:
-  assumes "m $ p1 = Some a"
-      and "p1 |\<notin>| s1"
-    shows "card ({0..length m} - insert p1 (fset s1)) < card ({0..length m} - fset s1)"
-proof -
-  have "card ({0..length m} - insert p1 (fset s1)) = card ({0..length m}) - card ({0..length m} \<inter> insert p1 (fset s1))"
-   and "card ({0..length m} - fset s1) = card ({0..length m}) - card ({0..length m} \<inter> (fset s1))" by (rule card_Diff_subset_Int, simp)+
-  moreover from assms(2) have "card ({0..length m} \<inter> insert p1 (fset s1)) = Suc (card ({0..length m} \<inter> (fset s1)))" using nth_safe_length[OF assms(1)] by simp
-  moreover have "card ({0..length m}) \<ge> card ({0..length m} \<inter> insert p1 (fset s1))" by (rule card_mono, auto)
-  ultimately show ?thesis by simp
-qed
-
-subsection \<open>Copy from Memory to Storage\<close>
-
-subsubsection \<open>Definition\<close>
-
-function copy_memory_storage_safe :: "location fset \<Rightarrow> ('a::address) memory \<Rightarrow> location \<Rightarrow> ('a::address) sdata option" where
-  "copy_memory_storage_safe s m l = 
-   (if l |\<in>| s then None else
-      case_memory m l
-        (\<lambda>v. Some (sdata.Value v))
-        (\<lambda>xs. those (map (copy_memory_storage_safe (finsert l s) m) xs) \<bind> Some \<circ> sdata.Array))"
-by pat_completeness auto
-termination
-  apply (relation "measure (\<lambda>(s,m,_). card ({0..length m} - fset s))")
-  using card_less_card by auto
-
-definition "copy_memory_storage = copy_memory_storage_safe {||}"
-
-subsubsection \<open>Examples\<close>
-
-lemma "P (copy_memory_storage mem_Array_2_3_true_false 8) = P (Some sd_Array_2_3_true_false)" by normalization
-
-subsection \<open>Copy from Memory to Calldata\<close>
-
-subsubsection \<open>Definition\<close>
-
-(*This is similar to memory storage. Can we use a type class to abstract it?*)
-function copy_memory_calldata_safe :: "location fset \<Rightarrow> ('a::address) memory \<Rightarrow> location \<Rightarrow> ('a::address) cdata option" where
-  "copy_memory_calldata_safe s m l = 
-   (if l |\<in>| s then None else
-      case_memory m l
-        (\<lambda>v. Some (cdata.Value v))
-        (\<lambda>xs. those (map (copy_memory_calldata_safe (finsert l s) m) xs) \<bind> Some \<circ> cdata.Array))"
-by pat_completeness auto
-termination
-  apply (relation "measure (\<lambda>(s,m,_). card ({0..length m} - fset s))")
-  using card_less_card by auto
-
-definition "copy_memory_calldata = copy_memory_calldata_safe {||}"
-
-subsubsection \<open>Examples\<close>
-
-lemma "P (copy_memory_storage mem_Array_2_3_true_false 8) = P (Some sd_Array_2_3_true_false)" by normalization
-
-subsection \<open>Copy from Storage to Memory\<close>
-
-subsubsection \<open>Definition\<close>
-
-function copy_storage_memory :: "(('a::address) sdata \<times> location) \<Rightarrow> ('a::address) memory \<Rightarrow> ('a::address) memory option" where
-  "copy_storage_memory (sdata.Value v, l) m = list_update_safe m l (mdata.Value v)"
-| "copy_storage_memory (sdata.Array xs, l) m =
-    case_memory m l
-      (K None)
-      (\<lambda>ys. if length xs = length ys then ofold copy_storage_memory (zip xs ys) m else None)"
-| "copy_storage_memory (sdata.Map _, _) _ = None"
-  by pat_completeness auto
-termination
-  apply (relation "measure (\<lambda>(s,b). size (fst s))") apply auto
-  by (metis less_irrefl_nat not_less_eq set_zip_leftD size_list_estimation)
-
-subsubsection \<open>Examples\<close>
-
-lemma "P (copy_storage_memory (sd_Array_2_3_true_false, 8) mem_Array_2_3_false_false) = P (Some (mem_Array_2_3_true_false))" by normalization
-
-
-subsection \<open>Copy from Calldata to Memory\<close>
-
-subsection \<open>Definition\<close>
-
-function copy_calldata_memory :: "(('a::address) cdata \<times> location) \<Rightarrow> ('a::address) memory \<Rightarrow> ('a::address) memory option" where
-  "copy_calldata_memory (cdata.Value v, l) m = list_update_safe m l (mdata.Value v)"
-| "copy_calldata_memory (cdata.Array xs, l) m =
-    case_memory m l
-      (K None)
-      (\<lambda>ys. if length xs = length ys then ofold copy_calldata_memory (zip xs ys) m else None)"
-  by pat_completeness auto
-termination
-  apply (relation "measure (\<lambda>(s,b). size (fst s))") apply auto
-  by (metis less_irrefl_nat not_less_eq set_zip_leftD size_list_estimation)
-
-fun copy_calldata_storage :: "('a::address) cdata \<Rightarrow> ('a::address) sdata" where
-  "copy_calldata_storage (cdata.Value v) = sdata.Value v"
-| "copy_calldata_storage (cdata.Array xs) = sdata.Array (map copy_calldata_storage xs)"
-
-subsection \<open>Examples\<close>
-
-section \<open>Stack\<close>
-
-subsection \<open>Definition\<close>
-
-datatype ('a::address) kdata =
-  Storage id "('a::address) valtype list" |
-  Memory location |
-  Calldata id "('a::address) valtype list" |
-  Value (vt: "('a::address) valtype")
+fun vtbytes_cast :: "nat \<Rightarrow> ('a::address) valtype \<Rightarrow> ('a::address) valtype option" where
+  "vtbytes_cast m (Bytes xs) = Some (Bytes (resize_list m (CHR 0x00) xs))"
+| "vtbytes_cast m _ = None"
 
 section \<open>State\<close>
 
 subsection \<open>Definition\<close>
 
-subsubsection \<open>Definition\<close>
-
-type_synonym 'a stack = "(id, 'a kdata) fmap"
+type_synonym 'v stack = "(id, 'v kdata) fmap"
 type_synonym 'a balances = "'a \<Rightarrow> nat"
-type_synonym 'a storage = "'a \<Rightarrow> id \<Rightarrow> 'a sdata"
-type_synonym 'a calldata = "(id, 'a cdata) fmap"
+type_synonym ('a, 'v) storage = "'a \<Rightarrow> id \<Rightarrow> 'v storage_data"
+type_synonym 'v calldata = "(id, 'v call_data) fmap"
 
 record ('a::address) state =
-  Memory:: "('a::address) memory"
-  Calldata:: "('a::address) calldata"
-  Storage:: "('a::address) storage"
-  Stack:: "('a::address) stack"
+  Memory:: "('a::address valtype) memory"
+  Calldata:: "('a::address valtype) calldata"
+  Storage:: "('a::address, 'a::address valtype) storage"
+  Stack:: "('a::address valtype) stack"
   Balances::"('a::address) balances"
+
+definition sameState where "sameState s s' \<equiv> state.Stack s' = state.Stack s \<and> state.Memory s' = state.Memory s \<and> state.Calldata s' = state.Calldata s"
 
 subsection \<open>Update Function\<close>
 
@@ -437,13 +171,16 @@ datatype ex = Err
 definition balances_update:: "('a::address) \<Rightarrow> nat \<Rightarrow> ('a::address) state \<Rightarrow> ('a::address) state" where
   "balances_update i n s = s\<lparr>Balances := (Balances s)(i := n)\<rparr>"
 
-definition calldata_update:: "id \<Rightarrow> ('a::address) cdata \<Rightarrow> ('a::address) state \<Rightarrow> ('a::address) state" where
+definition calldata_update:: "id \<Rightarrow> ('a::address valtype) call_data \<Rightarrow> ('a::address) state \<Rightarrow> ('a::address) state" where
   "calldata_update i d = Calldata_update (fmupd i d)"
 
-definition stack_update:: "id \<Rightarrow> ('a::address) kdata \<Rightarrow> ('a::address) state \<Rightarrow> ('a::address) state" where
+definition stack_update:: "id \<Rightarrow> ('a::address valtype) kdata \<Rightarrow> ('a::address) state \<Rightarrow> ('a::address) state" where
   "stack_update i d = Stack_update (fmupd i d)"
 
-definition memory_update:: "location \<Rightarrow> ('a::address) mdata \<Rightarrow> ('a::address) state \<Rightarrow> ('a::address) state" where
+definition memory_update:: "location \<Rightarrow> ('a::address valtype) mdata \<Rightarrow> ('a::address) state \<Rightarrow> ('a::address) state" where
   "memory_update i d s = s\<lparr>Memory := (Memory s)[i := d]\<rparr>"
+
+lemma balances_update_id[simp]: "balances_update x (Balances s x) s = s"
+  unfolding balances_update_def by simp
 
 end
